vera/VerilogToSMT/VerilogToSMT.v
@@ -6,6 +6,7 @@ From Stdlib Require Import Program.
 From Stdlib Require Import Psatz.
 From Stdlib Require Import String.
 From Stdlib Require Import ZArith.
+From Stdlib Require Import Sorting.Permutation.
 
 From Equations Require Import Equations.
 From ExtLib Require Import Data.List.
@@ -31,6 +32,8 @@ From vera Require Import SMTQueries.
 Import (coercions) VerilogSMTBijection.
 From vera Require Import Decidable.
 From vera Require Import Tactics.
+From vera Require VerilogSemantics.
+Import VerilogSemantics.Clean.
 
 Import ListNotations.
 Import CommonNotations.
@@ -252,14 +255,20 @@ Definition verilog_to_smt (name_tag : TaggedVariable.Tag) (var_start : nat) (vmo
     "Read from non-module-input"%string ;;
   assert_dec (all_vars_driven vmodule) "Undriven variables"%string ;;
   assert_dec
-    (list_subset (Verilog.module_body_writes (Verilog.modBody vmodule)) (Verilog.module_outputs vmodule))
-    "Non-output variables written to"%string ;;
-  assert_dec
     (NoDup (Verilog.module_body_writes (Verilog.modBody vmodule)))
     "Duplicate writes"%string ;;
   assert_dec
+    (NoDup (Verilog.module_outputs vmodule))
+    "Duplicate outputs"%string ;;
+  assert_dec
+    (Permutation (Verilog.module_body_writes (Verilog.modBody vmodule)) (Verilog.module_outputs vmodule))
+    "Non-output variables written to"%string ;;
+  assert_dec
     (VerilogSort.vmodule_sortable vmodule)
     "module is not sortable"%string ;;
+  assert_dec
+    (Forall clean_module_item_structure (Verilog.modBody vmodule))
+    "Invalid module item"%string ;;
   let var_assignment := assign_vars var_start (Verilog.modVariables vmodule) in
   let* nameMap := mk_bijection name_tag var_assignment in
   let* assertions :=
